Quicksort/Partition/Hoare/Eager/Lemmas.lean
@@ -30,7 +30,7 @@ private theorem hoare.eager.maybeSwap_sorted (as : Vector α n) (low high : Nat)
 include lt_asymm in
 include le_trans in
 private theorem hoare.eager.median_of_three_sorted {arr : Vector α n} {left mid right: Nat} (hlm : left ≤ mid) (hmr : mid ≤ right) (hr : right < n) :
-  let_fun arr_ := arr
+  have arr_ := arr
     |> (maybeSwap · ⟨left, by omega⟩ ⟨mid, by omega⟩)
     |> (maybeSwap · ⟨left, by omega⟩ ⟨right, by omega⟩)
     |> (maybeSwap · ⟨mid, by omega⟩ ⟨right, by omega⟩)
@@ -58,9 +58,9 @@ private theorem hoare.eager.median_of_three_sorted {arr : Vector α n} {left mid
     simp only [arr_]
     unfold maybeSwap
     split
-    · have : (arr2.swap ⟨mid, ‹_›⟩ ⟨right, ‹_›⟩)[left] = _ :=
-        arr2.getElem_swap_of_ne _ hleqm hlneqr
-      simp only [this, arr2.getElem_swap_left, Fin.getElem_fin]
+    · have : (arr2.swap mid right)[left] = arr2[left] :=
+        arr2.getElem_swap_of_ne hleqm hlneqr
+      simp only [this, arr2.getElem_swap_left]
       assumption
     · exact
       if hmeqr : mid = right then by
@@ -70,9 +70,9 @@ private theorem hoare.eager.median_of_three_sorted {arr : Vector α n} {left mid
         simp only [arr2]
         unfold maybeSwap
         split
-        · have : (arr1.swap ⟨left, by omega⟩ ⟨right, hr⟩)[mid] = _ :=
-            arr1.getElem_swap_of_ne (_ : mid < n) (Ne.symm hleqm) hmeqr
-          simp only [this, arr1.getElem_swap_left, Fin.getElem_fin]
+        · have : (arr1.swap left right)[mid] = _ :=
+            arr1.getElem_swap_of_ne (Ne.symm hleqm) hmeqr
+          simp only [this, arr1.getElem_swap_left]
           refine le_trans (lt_asymm ?_) hh1
           assumption
         · assumption
@@ -110,14 +110,14 @@ protected theorem hoare.eager.loop.permStabilizing {left right : Nat} {hr : righ
   · case case4 arr i j hli hjr hij hgt hh_ne hhne hlt ih =>
     apply PermStabilizing'.trans
     · apply PermStabilizing'.mono ih <;> omega
-    · apply swap_permStabilizing'; all_goals  simp only; omega
+    · apply swap_permStabilizing'; all_goals omega
   · case case5 arr i j hli hjr hij hgt hh_ne hhne hlt =>
     apply PermStabilizing'.refl
 
 
 protected theorem hoare.eager.permStabilizing {arr : Vector α n} {left : Nat} {right : Nat} {hlr : left < right} {hr : right < n} : PermStabilizing' left right (Partition.hoare.eager arr left right hlr hr).val.arr' arr := by
   apply PermStabilizing'.trans
-  · apply PermStabilizing'.mono hoare.eager.loop.permStabilizing <;> simp_arith
+  · apply PermStabilizing'.mono hoare.eager.loop.permStabilizing <;> omega
   ·
     -- apply sortAt_of_sortAt_of_sortAt_permStabilizing <;> omega
     apply PermStabilizing'.trans
@@ -218,8 +218,8 @@ protected theorem hoare.eager.sorted {arr : Vector α n} {left : Nat} {right : N
 
     have : PermStabilizing' (left + 1) (right - 1) x.arr' arr_ := hoare.eager.loop.permStabilizing
     replace hh2 : ¬lt pivot x.arr'[left] ∧ ¬lt x.arr'[right] pivot := by
-      have heq_left : x.arr'[left] = arr_[left] := this.2.1 ⟨left, by omega⟩ (by simp_arith)
-      have heq_right : x.arr'[right] = arr_[right] := this.2.2 ⟨right, by omega⟩ (by simp_arith; omega)
+      have heq_left : x.arr'[left] = arr_[left] := this.2.1 ⟨left, by omega⟩ (by grind)
+      have heq_right : x.arr'[right] = arr_[right] := this.2.2 ⟨right, by omega⟩ (by grind)
       rwa [heq_left, heq_right]
 
     have hh1_right : RangeHas n (¬lt x.arr'[·]  pivot) (x.j' + 1) right := by
