Quicksort/Partition/Lomuto/Lemmas.lean
@@ -11,32 +11,40 @@ include lt_asymm in
 private theorem lt_irrefl : ∀ (x : α), ¬lt x x :=
   fun _ h => (lt_asymm h) h
 
-
-
 protected theorem lomuto.loop.partition_bounds {left right : Nat}  {hlr : left < right} {hr : right < n} {pivot : α} {arr : Vector α n} {i j : Nat} {hli : left ≤ i} {hij : i ≤ j} {hjr : j ≤ right} : (loop left right hlr hr pivot arr i j hli hij hjr).val.j' < (loop left right hlr hr pivot arr i j hli hij hjr).val.i' := by
-  fun_induction lomuto.loop; all_goals
-    simp [*]; try omega
+  induction arr, i, j, hli, hij, hjr using lomuto.loop.induct (hr := hr) (pivot := pivot)  with
+  | case1 arr i j hli hij hjr' hjr hhlt ih  =>
+    unfold loop; simp [*]
+  | case2 arr i j hli hij hjr' hjr hhle ih =>
+    unfold loop; simp [*]
+  | case3 arr i j hli hij hjr' hjr =>
+    unfold loop; simp [*]
+    omega
 
 protected theorem lomuto.partition_bounds {arr : Vector α n} {left : Nat} {right : Nat} {hlr : left < right} {hr : right < n} : (lomuto arr left right hlr hr).val.j' < (lomuto arr left right hlr hr).val.i' := by
   unfold lomuto
   apply lomuto.loop.partition_bounds
 
-
-#check lomuto.loop.induct
-
 protected theorem lomuto.loop.permStabilizing {left right : Nat} {hlr : left < right} {hr : right < n} {pivot : α} {arr : Vector α n} {i j : Nat} {hli : left ≤ i} {hij :  i ≤ j} {hjr : j ≤ right} : PermStabilizing' i right (loop left right hlr hr pivot arr i j hli hij hjr).val.arr' arr
 := by
-  fun_induction lomuto.loop with
+  induction arr, i, j, hli, hij, hjr using lomuto.loop.induct (hr := hr) (pivot := pivot) with
   | case1 arr i j hli hij hjr' hjr hhlt ih  =>
+    unfold loop; simp [*]
+
     apply PermStabilizing'.trans
     · apply PermStabilizing'.mono ih <;> omega
-    · apply swap_permStabilizing' <;> omega
+    · apply swap_permStabilizing' <;>  omega
   | case2 arr i j hli hij hjr' hjr hhle ih =>
-    simp only [ih]
+    unfold loop; simp [*]
+
   | case3 arr i j hli hij hjr' hjr =>
+    unfold loop; simp [*]
+
+    have : right = j  := by omega
+    suffices PermStabilizing' i right (arr.swap i j) arr by grind
+
     apply swap_permStabilizing'
     all_goals omega
-
 
 
 -- set_option trace.profiler true in
@@ -69,11 +77,10 @@ private theorem _root_.Vector.inclusive_swap {arr : Vector α n} {i j : Nat} {hi
     · simp only [Fin.getElem_fin, arr.getElem_swap_right]
       exact this.1
     · intro p _ _
-      simp only [Fin.getElem_fin,
+      simp only [arr',
         show arr'[p] = _ by
           apply arr.getElem_swap_of_ne; all_goals simp; omega]
-      -- apply this.2; all_goals omega
-      sorry
+      apply this.2; all_goals omega
 
 section split_ih
 variable {a b p q : Prop} (ih : a → b → c → p ∧ q) include ih
@@ -81,90 +88,92 @@ private theorem _root_.split_ih_left : a → b → c → p := (ih · · · |>.le
 private theorem _root_.split_ih_right :  a → b → c → q := (ih · · · |>.right)
 end split_ih
 
+
+
 variable (lt_asymm : ∀ {x y : α}, lt x y → ¬lt y x)
 
-set_option tactic.fun_induction.unfolding false in
+
 include lt_asymm in
 -- protected theorem lomuto.loop.sorted {left right : Nat} {hr : right < n} {pivot : α} {arr : Vector α n} {i j : Nat} {hli : left ≤ i} {hij :  i ≤ j} {hjr : j ≤ right} (hxij : i < j → RangeHas n (¬lt arr[·] pivot) i j ) (hxr : ¬lt arr[right] pivot) (hxr' : ¬lt pivot arr[right]) : let x := (loop left right hr pivot arr i j hli hij hjr).val; RangeHas n (¬lt pivot x.arr'[·]) i x.i' ∧  RangeHas n (¬lt x.arr'[·] pivot) (x.j' + 1) (right + 1) := by
 protected theorem lomuto.loop.sorted {left right : Nat} {hlr : left < right} {hr : right < n} {pivot : α} {arr : Vector α n} {i j : Nat} {hli : left ≤ i} {hij :  i ≤ j} {hjr : j ≤ right} (hxij : i < j → RangeHas n (¬lt arr[·] pivot) i j ) (hxr : ¬lt arr[right] pivot) (hxr' : ¬lt pivot arr[right]) : IsPartitioned i right pivot (loop left right hlr hr pivot arr i j hli hij hjr).val := by
-  sorry
-  -- fun_induction lomuto.loop with
-  -- | case1 arr i j hli hij hjr' hjr hhlt ih =>
-  --   unfold loop; simp [-Fin.getElem_fin, *]
-  --   have hi : i < n := by omega
-  --   have hj : j < n := by omega
-  --   rw [Nat.add_lt_add_iff_right] at ih
-  --   let i_fin : Fin n := ⟨i, hi⟩
-  --   let j_fin : Fin n := ⟨j, hj⟩
 
-  --   constructor
-  --   apply RangeHas.prepend (ha := hi) (pred := (¬lt _ _[·] = _))
-  --   · let x : Partition α n := (loop left right hlr hr pivot (arr.swap i j) (i + 1) (j + 1) (by omega) (by omega) (by omega)).val
-  --     have hperm : PermStabilizing' _ _ x.arr' _ := lomuto.loop.permStabilizing
-  --     simp only [hperm.2.1 i_fin (by simp only [i_fin] ; omega), Fin.getElem_fin, arr.getElem_swap_left]
-  --     exact lt_asymm hhlt
+  induction arr, i, j, hli, hij, hjr using lomuto.loop.induct (hr := hr) (pivot := pivot) with
+  | case1 arr i j hli hij hjr' hjr hhlt ih =>
+    let i_fin : Fin n := ⟨i, by omega⟩
+    unfold loop; simp [-Fin.getElem_fin, *]
+    have hi : i < n := by omega
+    have hj : j < n := by omega
+    rw [Nat.add_lt_add_iff_right] at ih
+    let j_fin : Fin n := ⟨j, hj⟩
 
-  --   all_goals
-  --     intro _ _ _
-  --     try apply split_ih_left ih
-  --     try apply split_ih_right ih
-  --     any_goals simp only [i_fin]
-  --     any_goals omega
-  --     · intro hij'
-  --       simp only [Vector.inclusive_swap hij']
-  --       exact hxij hij'
-  --     · simp only [Fin.getElem_fin, show (arr.swap ⟨i, by omega⟩ ⟨j, by omega⟩)[right] = _ by
-  --         apply arr.getElem_swap_of_ne; all_goals simp; omega]
-  --       exact hxr
-  --     · simp only [Fin.getElem_fin, show (arr.swap ⟨i, by omega⟩ ⟨j, by omega⟩)[right] = _ by
-  --         apply arr.getElem_swap_of_ne; all_goals simp; omega]
-  --       exact hxr'
+    constructor
+    apply RangeHas.prepend (ha := hi) (pred := (¬lt _ _[·] = _))
+    · let x : Partition α n := (loop left right hlr hr pivot (arr.swap i j (by omega) (by omega)) (i + 1) (j + 1) (by omega) (by omega) (by omega)).val
+      have hperm : PermStabilizing' _ _ x.arr' _ := lomuto.loop.permStabilizing
+      simp only [x, show x.arr'[i] = (arr.swap i j hi hj)[i] from  hperm.2.1 i_fin (by grind), Fin.getElem_fin, arr.getElem_swap_left]
+      exact lt_asymm hhlt
 
-  -- | case2 arr i j hli hij hjr' hjr hhle ih =>
-  --   unfold loop; simp [-Fin.getElem_fin, *]
-  --   have hj : j < n := by omega
+    all_goals
+      intro _ _ _
+      try apply split_ih_left ih
+      try apply split_ih_right ih
+      -- any_goals simp only [i_fin]
+      any_goals omega
+      · intro hij'
+        simp only [Vector.inclusive_swap hij']
+        exact hxij hij'
+      · simp only [show (arr.swap i j)[right] = _ by
+          apply arr.getElem_swap_of_ne; all_goals simp; omega]
+        exact hxr
+      · simp only [show (arr.swap i j)[right] = _ by
+          apply arr.getElem_swap_of_ne; all_goals simp; omega]
+        exact hxr'
 
-  --   constructor; all_goals
-  --   intro _ _ _
-  --   try apply split_ih_right ih
-  --   try apply split_ih_left ih
-  --   any_goals omega
-  --   · intro _
-  --     cases Nat.eq_or_lt_of_le hij with
-  --     | inr hlt =>
-  --       apply RangeHas.append hhle (hxij hlt) (hb := hj)
-  --     | inl heq =>
-  --       rw [heq]
-  --       intro k _ _
-  --       simpa only [Fin.getElem_fin, (by omega : k = j)]
-  --   · exact hxr
-  --   · exact hxr'
+  | case2 arr i j hli hij hjr' hjr hhle ih =>
+    unfold loop; simp [-Fin.getElem_fin, *]
+    have hj : j < n := by omega
 
-  -- | case3 arr i j hli hij _ _ =>
-  --   unfold loop; simp [-Fin.getElem_fin, *]
-  --   have hi : i < n := by omega
+    constructor; all_goals
+    intro _ _ _
+    try apply split_ih_right ih
+    try apply split_ih_left ih
+    any_goals omega
+    · intro _
+      cases Nat.eq_or_lt_of_le hij with
+      | inr hlt =>
+        apply RangeHas.append hhle (hxij hlt) (hb := hj)
+      | inl heq =>
+        rw [heq]
+        intro k _ _
+        simpa only [Fin.getElem_fin, (by omega : k = j)]
+    -- · exact hxr
+    -- · exact hxr'
 
-  --   constructor
-  --   · simp only [Fin.getElem_fin]
-  --     simpa only [RangeHas.singular (h := hi), arr.getElem_swap_left]
-  --   · have hrj : j = right := by omega
-  --     subst hrj
-  --     suffices RangeHas n (¬lt (arr.swap ⟨i, hi⟩ ⟨j, hr⟩)[·] pivot) i (j + 1) by
-  --       change RangeHas n (¬lt (arr.swap ⟨i, hi⟩ ⟨j, hr⟩)[·] pivot) (i - 1 + 1) (j + 1)
-  --       apply RangeHas.mono this <;> omega
+  | case3 arr i j hli hij _ _ =>
+    unfold loop; simp [-Fin.getElem_fin, *]
+    have hi : i < n := by omega
 
-  --     cases Nat.eq_or_lt_of_le hij with
-  --     | inr hlt =>
-  --       apply RangeHas.mono
-  --       show RangeHas _ _ i (j + 1)
-  --       apply RangeHas.prepend (ha := hi) (pred := (¬lt _[·] _ = _))
-  --       · simpa only [Fin.getElem_fin, arr.getElem_swap_left]
-  --       · simp only [Vector.inclusive_swap (hi := hi) (hj := hr) hlt]
-  --         exact hxij hlt
-  --       all_goals omega
-  --     | inl heq =>
-  --       simp only [Fin.getElem_fin]
-  --       simpa only [heq, getElem_swap, RangeHas.singular (h := hr), ne_eq]
+    constructor
+    · simp only [Fin.getElem_fin]
+      simpa only [RangeHas.singular (h := hi), arr.getElem_swap_left]
+    · have hrj : j = right := by omega
+      subst hrj
+      suffices RangeHas n (¬lt (arr.swap i j)[·] pivot) i (j + 1) by
+        change RangeHas n (¬lt (arr.swap i j)[·] pivot) (i - 1 + 1) (j + 1)
+        apply RangeHas.mono this <;> omega
+
+      cases Nat.eq_or_lt_of_le hij with
+      | inr hlt =>
+        apply RangeHas.mono
+        show RangeHas _ _ i (j + 1)
+        apply RangeHas.prepend (ha := hi) (pred := (¬lt _[·] _ = _))
+        · simpa only [Fin.getElem_fin, arr.getElem_swap_left]
+        · simp only [Vector.inclusive_swap (hi := hi) (hj := hr) hlt]
+          exact hxij hlt
+        all_goals omega
+      | inl heq =>
+        simp only [Fin.getElem_fin]
+        grind only [getElem_swap]
 
 
 variable (le_trans : ∀ {x y z : α}, ¬lt y x → ¬lt z y → ¬lt z x)
